The following is an example of an embedding from a CLTS control problem into an FDS control problem, for which a strategy is built, converted into an FDS controller and then translated into a CLTS controller. 

The CLTS control problem tries to process two items before resetting the system. The initial state requires that the environment signals that the conditions are met through the action $r$ (ready) otherwise it will keep informing that the status is pending through action $p$.  The system can then process an item through action $P$ or issue a reset $R$. Proposition $e$ indicates that an enabled state has been reached after which the processing can start, propositions $a$ and $b$ denote that the first and second items respectively have been processed. 
The property to be satisfied is captured by $\varphi: \square \Diamond e$ $\implies$ $(\square \Diamond a$ $\wedge$ $\square \Diamond b)$. The CLTS control problem will be $\mathcal{I}=\langle E, \{P,R\}, \varphi \rangle$ with $E$ being the automaton depicted in Figure ~\ref{fig:clts_to_fds_E}. The labels next to the state numbers indicate which propositions hold at any given point.

\begin{figure}[bt]
	\centering
	%\minipage{0.32\textwidth}%
	%\centering
	\VCDraw{
	\begin{VCPicture}{(-2.5,-1)(2.5,3.5)}
		\SetStateLabelScale{1}
		\SetEdgeLabelScale{1.2}
		\State[0:-]{(-2,2.3)}{0}
		\State[1:e]{(2,2.3)}{1}
		\State[2:a]{(2,-0.3)}{2}
		\State[3:b]{(-2,-0.3)}{3}
		\Initial[w]{0}
		\ArcL{0}{1}{<r>}        
		\ArcL{1}{0}{<R>}        
		\LoopN{0}{<p>}		
		\ArcL{1}{2}{<P>}        
		\ArcL{2}{0}{<R>}        				
		\ArcL{2}{3}{<P>}        
		\ArcL{3}{0}{<R>}        						
	\end{VCPicture}
	}
	\caption{Automaton $E$ from $\mathcal{I}=\langle E, \{P,R\}, \varphi \rangle$}
	\label{fig:clts_to_fds_E}
	%\endminipage\hfill
\end{figure}

The FDS equivalent formula to $E$ is built using the translation proposed before, with $\gsX$ being the set $\{\hat{p},\hat{r}\}$ and $\gsY$ being $\{s_0,s_1,\hat{P},\hat{R},\hat{e},\hat{a},\hat{b}\}$. Then we have:

\footnotesize
\vspace{1em}
\begin{tabular}{ r c l }
	$\theta_{e}$ &$=$& $\bar{\hat{p}} \wedge \bar{\hat{r}}$\\
	$\theta_{s}$ &$=$& $\bar{s_0} \wedge \bar{s_1} \wedge \bar{\hat{P}} \wedge \bar{\hat{R}} \wedge \bar{\hat{e}} \wedge \bar{\hat{a}} \wedge \bar{\hat{b}}$\\	
	$\rho_{env.enabling}$ &$=$& $((\bar{s_0} \wedge \bar{s_1} ) \implies ((\hat{p} \wedge \bar{\hat{r}}) \vee (\bar{\hat{p}} \wedge \hat{r}))) \wedge$\\
	&& $((s_0 \vee s_1 ) \implies (\bar{\hat{p}} \wedge \bar{\hat{r}}))$\\	
	$\rho_{sys.enabling}$ &$=$& $((\bar{s_0} \wedge \bar{s_1} ) \implies (\bar{\hat{P}} \wedge \bar{\hat{R}})) \wedge$\\
	&& $((s_0 \vee s_1 ) \implies ((\hat{P} \wedge \bar{\hat{R}}) \vee (\bar{\hat{P}} \wedge  \hat{R})))$\\		
	$\rho_{update.states}$ &$=$& $((\bar{s_0} \wedge \bar{s_1} \wedge \hat{p} \wedge \bar{\hat{r}} \wedge \bar{\hat{P}} \wedge \bar{\hat{R}}) \implies (\bar{s_0}' \wedge \bar{s_1}')) \wedge$\\
	&&$((\bar{s_0} \wedge \bar{s_1} \wedge \bar{\hat{p}} \wedge \hat{r} \wedge \bar{\hat{P}} \wedge \bar{\hat{R}}) \implies (s_0' \wedge \bar{s_1}')) \wedge$\\	
	&&$((s_0 \wedge \bar{s_1} \wedge \bar{\hat{p}} \wedge \bar{\hat{r}} \wedge \bar{\hat{P}} \wedge \hat{R}) \implies (\bar{s_0}' \wedge \bar{s_1}')) \wedge$\\	
	&&$((s_0 \wedge \bar{s_1} \wedge \bar{\hat{p}} \wedge \bar{\hat{r}} \wedge \hat{P} \wedge \bar{\hat{R}}) \implies (\bar{s_0}' \wedge s_1')) \wedge$\\	
	&&$((\bar{s_0} \wedge s_1 \wedge \bar{\hat{p}} \wedge \bar{\hat{r}} \wedge \bar{\hat{P}} \wedge \hat{R}) \implies (\bar{s_0}' \wedge \bar{s_1}')) \wedge$\\		
	&&$((\bar{s_0} \wedge s_1 \wedge \bar{\hat{p}} \wedge \bar{\hat{r}} \wedge \hat{P} \wedge \bar{\hat{R}}) \implies (s_0' \wedge s_1')) \wedge$\\		
	&&$((s_0 \wedge s_1 \wedge \bar{\hat{p}} \wedge \bar{\hat{r}} \wedge \bar{\hat{P}} \wedge \hat{R}) \implies (\bar{s_0}' \wedge \bar{s_1}'))$\\	
	$\rho_{update.propositions}$ &$=$& $((\bar{s_0} \wedge \bar{s_1}) \implies (\bar{\hat{e}}' \wedge \bar{\hat{a}}' \wedge \bar{\hat{b}}')) \wedge$\\
	&& $((s_0 \wedge \bar{s_1}) \implies (\hat{e}' \wedge \bar{\hat{a}}' \wedge \bar{\hat{b}}')) \wedge$\\
	&& $((\bar{s_0} \wedge s_1) \implies (\bar{\hat{e}}' \wedge \hat{a}' \wedge \bar{\hat{b}}')) \wedge$\\
	&& $((s_0 \wedge s_1) \implies (\bar{\hat{e}}' \wedge \bar{\hat{a}}' \wedge \hat{b}'))$\\	
	$\gsRhoE$&$=$&$\rho_{env.enabling}$\\		
	$\gsRhoS$&$=$&$\rho_{sys.enabling} \wedge  \rho_{update.states} \wedge  \rho_{update.propositions}$\\	
\end{tabular}
\vspace{1em}
\normalsize

If we keep only the behavior that conforms to $\theta_e, \theta_s, \rho_e$ and $\rho_s$ this translation induces the Kripke automaton depicted in Figure ~\ref{fig:clts_to_fds_K}.

\begin{figure}[bt]
	\centering
	%\minipage{0.32\textwidth}%
	%\centering
	\VCDraw{
		\begin{VCPicture}{(-6.5,-2.5)(6.5,3.5)}
			\SetStateLabelScale{1}
			\SetEdgeLabelScale{1.2}
			\StateVar[0:\overline{s_0 s_1 e a b}p\overline{r P R}]{(-6,-0.3)}{0}
			\StateVar[1:\overline{s_0 s_1 e a b p}r\overline{P R}]{(-6,2.3)}{1}
			\StateVar[2:s_0\overline{s_1 e a b p r P} R]{(-2,-0.3)}{2}
			\StateVar[3:s_0\overline{s_1 e a b p r} P \overline{R}]{(-2,2.3)}{3}
			\StateVar[4:\overline{s_0}s_1 \overline{e a b p r P} R]{(2,-0.3)}{4}
			\StateVar[5:\overline{s_0}s_1 \overline{e a b p r} P \overline{R}]{(2,2.3)}{5}			
			\StateVar[6:s_0 s_1\overline{e a b p r P} R]{(6,1)}{6}						
			\Initial[w]{0}
			\Initial[w]{1}
			\LoopS{0}{}			
			\EdgeL{0}{1}{}        
			\EdgeL{1}{3}{}        
			\EdgeL{2}{1}{}        			
			\EdgeL{2}{0}{}        						
			\EdgeL{3}{5}{}        
			\EdgeL{4}{1}{}        			
			\ArcL{4}{0}{}        						
			\EdgeL{5}{6}{}        			
			\VArcR[.5]{arcangle=45,ncurv=.6}{6}{0}{}        						
			\VArcL[.5]{arcangle=-45,ncurv=.6}{6}{1}{}        									
		\end{VCPicture}
	}
	\caption{Kripke structure induced from $\theta$ and $\rho$}
	\label{fig:clts_to_fds_K}
	%\endminipage\hfill
\end{figure}

Explain winning states, strat, restriction, explain out of $\rho_e$ is arbitrary.

Strategy as mapping.

Restriction as Kripke.

\begin{figure}[bt]
	\centering
	%\minipage{0.32\textwidth}%
	%\centering
	\VCDraw{
		\begin{VCPicture}{(-6.5,-2.5)(6.5,3.5)}
			\SetStateLabelScale{1}
			\SetEdgeLabelScale{1.2}
			\StateVar[0:\overline{s_0 s_1 e a b}p\overline{r P R}]{(-6,-0.3)}{0}
			\StateVar[1:\overline{s_0 s_1 e a b p}r\overline{P R}]{(-6,2.3)}{1}
			\StateVar[3:s_0\overline{s_1 e a b p r} P \overline{R}]{(-2,2.3)}{3}
			\StateVar[5:\overline{s_0}s_1 \overline{e a b p r} P \overline{R}]{(2,2.3)}{5}			
			\StateVar[6:s_0 s_1\overline{e a b p r P} R]{(6,1)}{6}						
			\Initial[w]{0}
			\Initial[w]{1}
			\LoopS{0}{}			
			\EdgeL{0}{1}{}        
			\EdgeL{1}{3}{}        
			\EdgeL{3}{5}{}        
			\EdgeL{5}{6}{}        			
			\VArcR[.5]{arcangle=45,ncurv=.6}{6}{0}{}        						
			\VArcL[.5]{arcangle=-45,ncurv=.6}{6}{1}{}        									
		\end{VCPicture}
	}
	\caption{Kripke structure induced from $\theta$ and $\rho$ after strengthening with $\hat{f}$}
	\label{fig:clts_to_fds_F}
	%\endminipage\hfill
\end{figure}

Explain translation back to CLTS controller.

\begin{figure}[H]
	\centering
	%\minipage{0.32\textwidth}%
	%\centering
	\VCDraw{
		\begin{VCPicture}{(-2.5,-1)(2.5,3.5)}
			\SetStateLabelScale{1}
			\SetEdgeLabelScale{1.2}
			\State[0]{(-2,2.3)}{0}
			\State[1]{(2,2.3)}{1}
			\State[2]{(2,-0.3)}{2}
			\State[3]{(-2,-0.3)}{3}
			\Initial[w]{0}
			\ArcL{0}{1}{<r>}        
			\LoopN{0}{<p>}		
			\ArcL{1}{2}{<P>}        
			\ArcL{2}{3}{<P>}        
			\ArcL{3}{0}{<R>}        						
		\end{VCPicture}
	}
	\caption{Controller $C$ translated from $\fdsD$}
	\label{fig:clts_to_fds_C}
	%\endminipage\hfill
\end{figure}